If we substitute \( e^{i \pi} = -1 \) in place of \( \pi \), we can rewrite the formula for the radius \( r \) in terms of the circumference \( C \) as follows:

1. Start with the original formula:
   \[
   r = \frac{C}{2\pi}
   \]

2. Substitute \( \pi = i \ln(-1) \), based on \( e^{i \pi} = -1 \), which implies that \( \pi = i \ln(-1) \):
   \[
   r = \frac{C}{2 \cdot i \ln(-1)}
   \]

### Interpretation
With this substitution, the formula for the radius \( r \) becomes more complex because we're introducing complex numbers into the expression. However, this substitution is more of a theoretical manipulation and does not simplify the radius in a practical way.

In practical terms, \( \pi \) is generally retained in the formula because it is a real constant, whereas substituting \( e^{i \pi} = -1 \) is mostly used in complex analysis and theoretical contexts where the relationship \( e^{i \pi} + 1 = 0 \) is relevant.

