([README-any-base.md](https://t2m.io/c0ec7AD))
---
Yes, the transformation of equations like \( f = g + m_1 + m_2 - 2r \) in the **exponent space** can apply to **any base**, not just powers of 2. Here's why:

---

### **Key Idea: Represent Numbers as Powers of a Base**
In any base \(b\):
- A number \(x\) can be represented as \(b^n\), where \(n\) is the logarithm of \(x\) in base \(b\): \(n = \log_b(x)\).
- Using this representation, multiplication and division of numbers correspond to **addition and subtraction** of their exponents in that base.

For example, in base \(b\):
1. Multiplication:
   \[
   x \cdot y = b^n \cdot b^m = b^{n + m}.
   \]
2. Division:
   \[
   \frac{x}{y} = \frac{b^n}{b^m} = b^{n - m}.
   \]

---

### **Rewriting \(F = G \frac{m_1 m_2}{r^2}\) in Any Base**

1. **Represent Each Variable in Exponent Space**:
   \[
   F = b^f, \quad G = b^g, \quad m_1 = b^{m_1}, \quad m_2 = b^{m_2}, \quad r = b^r.
   \]

2. **Substitute into the Formula**:
   \[
   b^f = b^g \cdot \frac{b^{m_1} \cdot b^{m_2}}{(b^r)^2}.
   \]

3. **Simplify Using Exponent Rules**:
   - \(b^a \cdot b^b = b^{a+b}\),
   - \(b^a / b^b = b^{a-b}\),
   - \((b^a)^2 = b^{2a}\).

   The equation becomes:
   \[
   b^f = b^g \cdot b^{m_1 + m_2} \cdot b^{-2r}.
   \]

4. **Combine Exponents**:
   \[
   b^f = b^{g + m_1 + m_2 - 2r}.
   \]

5. **Equate the Exponents**:
   Since the bases are the same, equate the exponents:
   \[
   f = g + m_1 + m_2 - 2r.
   \]

---

### **Conclusion**
This simplification works for **any base** because the core operations (multiplication and division) transform into addition and subtraction in the **logarithmic representation**. Whether the base is \(2\), \(10\), \(16\), or any other number, the formula simplifies to a linear relationship in the exponent space:

\[
f = g + m_1 + m_2 - 2r.
\]


---

[README-lortentz.md](https://t2m.io/TQbtZRJ)
