([README-rewrite-f.md](https://t2m.io/3yrqmWP))
---
In the context of a numbering system where all numbers are represented as powers of 2, let's rewrite the formula for gravitational force:

\[
F = G \frac{m_1 m_2}{r^2}
\]

where:
- \(F\): Force
- \(G\): Gravitational constant
- \(m_1, m_2\): Masses
- \(r\): Distance between the masses

### **Step 1: Represent Variables as Powers of 2**
In the \(2^N\) system:
- Each variable (e.g., \(F, G, m_1, m_2, r\)) is expressed as a power of 2.
- Let:
  \[
  F = 2^{f}, \quad G = 2^{g}, \quad m_1 = 2^{m_1}, \quad m_2 = 2^{m_2}, \quad r = 2^{r}.
  \]

### **Step 2: Rewrite the Formula**
Substitute the power-of-2 representations into the formula:
\[
2^f = 2^g \cdot \frac{2^{m_1} \cdot 2^{m_2}}{(2^r)^2}.
\]

### **Step 3: Simplify Using Exponent Rules**
Apply the rules for powers of 2:
- \(2^a \cdot 2^b = 2^{a+b}\),
- \(2^a / 2^b = 2^{a-b}\),
- \((2^a)^2 = 2^{2a}\).

Simplify the equation:
\[
2^f = 2^g \cdot 2^{m_1 + m_2} \cdot 2^{-2r}.
\]

Combine exponents:
\[
2^f = 2^{g + m_1 + m_2 - 2r}.
\]

### **Step 4: Equate the Exponents**
Since the left-hand side is \(2^f\), equate the exponents:
\[
f = g + m_1 + m_2 - 2r.
\]

### **Final Formula in Exponent Space**
\[
f = g + m_1 + m_2 - 2r.
\]

---

### **Interpretation**
In the \(2^N\) system, the gravitational force equation simplifies to a **linear relationship between the exponents** of the variables. This highlights the elegance of the power-of-2 system: multiplication and division in the original formula reduce to addition and subtraction of exponents.


---

[README-any-base.md](https://t2m.io/c0ec7AD)
