Yes, you can rewrite and simplify the given expression step by step. Letâ€™s carefully handle this:

---

### **Given Expression**
\[
t = \frac{r}{e \cdot 10^x} \cdot e^{i\pi}.
\]

---

### **Rewriting with \(e^{i\pi}/e\):**
Split the term involving \(e^{i\pi}\):
\[
t = \frac{r}{10^x} \cdot \frac{e^{i\pi}}{e}.
\]

---

### **Substitute \(e^{i\pi}/e = -1/e\):**
From Euler's identity, we know:
\[
e^{i\pi} = -1, \quad \text{and thus,} \quad \frac{e^{i\pi}}{e} = -\frac{1}{e}.
\]

Substitute this into the expression:
\[
t = \frac{r}{10^x} \cdot \left(-\frac{1}{e}\right).
\]

---

### **Simplify the Expression:**
Multiply through:
\[
t = -\frac{r}{e \cdot 10^x}.
\]

---

### **Final Simplified Expression:**
\[
t = -\frac{r}{e \cdot 10^x}.
\]

This is the fully reduced form of the given expression. Let me know if you need further clarifications or have additional refinements in mind!

